---
title: "Empirical Likelihood Algorithms"
author: "Shimeng Huang, Martin Lysy"
date: "`r Sys.Date()`"
output:
  bookdown::html_vignette2:
    toc: true
vignette: >
  %\VignetteIndexEntry{Empirical Likelihood Algorithms}
  %\VignetteEngine{knitr::rmarkdown}
  %\VignetteEncoding{UTF-8}
bibliography: flexEL.bib
---

<!-- <script type="text/x-mathjax-config"> -->
<!-- MathJax.Hub.Config({ -->
<!--   TeX: { equationNumbers: { autoNumber: "AMS" } } -->
<!-- }); -->
<!-- </script> -->

\DeclareMathOperator*{\argmax}{arg\,max}
\DeclareMathOperator*{\argmin}{arg\,min}
\DeclareMathOperator{\EL}{EL}
\DeclareMathOperator{\CEL}{CEL}
\newcommand{\SCEL}{\textrm{SCEL}}
\newcommand{\bm}[1]{\boldsymbol{#1}}
\newcommand{\bz}{{\bm{0}}}
\newcommand{\bg}{{\bm{g}}}
\newcommand{\bG}{{\bm{G}}}
\newcommand{\XX}{{\bm{X}}}
\newcommand{\xx}{{\bm{x}}}
\newcommand{\zz}{{\bm{z}}}
\newcommand{\bbe}{{\bm{\beta}}}
\newcommand{\tta}{{\bm{\tau}}}
\newcommand{\bga}{{\bm{\gamma}}}
\newcommand{\bla}{{\bm{\lambda}}}
\newcommand{\w}{{\omega}}
\newcommand{\oom}{{\bm{\omega}}}
\newcommand{\eps}{{\epsilon}}
\newcommand{\eep}{{\bm{\epsilon}}}
\newcommand{\ee}{{\bm{e}}}
\newcommand{\tth}{{\bm{\theta}}}
\newcommand{\E}{\textrm{E}}
\newcommand{\F}{\textrm{F}}
\newcommand{\R}{\mathbb R}
\newcommand{\var}{\textrm{var}}
\newcommand{\iid}{\stackrel {\textrm{iid}}{\sim}}
\newcommand{\ind}{\stackrel {\textrm{ind}}{\sim}}
\newcommand{\N}{\mathcal N}
\newcommand{\ud}{\mathop{}\!\mathrm{d}}
\newcommand{\dth}{\frac{\ud}{\ud\tth}}
\DeclareMathOperator{\indicator}{\mathbb{1}}
\DeclareMathOperator{\indsmooth}{\mathcal{S}}
\newcommand{\indexset}{\mathcal{I}}
\newcommand{\simplex}{\Delta}
\DeclareMathOperator{\categorical}{Categorical}
\DeclareMathOperator{\bernoulli}{Bernoulli}

# General Empirical Likelihood

Suppose we have iid observations $\xx_1, \ldots \xx_n \iid F(\xx \mid \tth)$.  The goal is to estimate the model parameters $\tth$.  However, the complete parametric specification of $F(\xx \mid \tth)$ is unknown.  Instead, we only have the moment conditions
$$
E[\bg(\xx, \tth)] = \bz.
$$
The empirical likelihood (EL) function is defined as
$$
\log \EL(\tth) = \log \EL(\tth, \hat \oom) =  \sum_{i=1}^n \log \hat \omega_i,
$$
where $\hat \oom = \hat \oom(\tth)$ solves the optimization problem
\begin{equation}
\max_{\oom} \log \EL(\tth, \oom) \qquad \Big\vert \qquad \sum_{i=1}^n \omega_i \cdot \bg_i = \bz, \quad \oom \in \simplex^{n-1},
(\#eq:elopt)
\end{equation}
where $\bg_i = \bg(\xx_i, \tth) \in \mathbb R^m$ and 
$$
\simplex^{n-1} = \{\oom \in \mathbb R^n: \sum_{i=1}^n \omega_i = 1, \omega_i > 0\}
$$ 
is the $(n-1)$-dimensional probability simplex.  The estimator $\hat \tth = \argmax_{\tth} \log \EL(\tth)$ is called the EL estimator of $\tth$.

## Computation

For fixed $\tth$, we may solve the optimization problem \@ref(eq:elopt) as follows.  First, let us consider solving \@ref(eq:elopt) for a slighly generalized "weighted" EL function
\begin{equation}
\log \EL(\tth, \oom) = \sum_{i=1}^n q_i \log \omega_i,
(\#eq:wel)
\end{equation}
where $q_i > 0$ are the weights.  Let $r_i = q_i / \sum_{i=1}^n q_i$, and consider the convex function
$$
Q(\bla) = \sum_{i=1}^n r_i \log^\star\left(1 - \bla'\bg_i; r_i\right),
$$
where
$$
\log^\star(x; r) = 
\begin{cases} 
\log(x) & x \ge r \\
- \tfrac 1 2 (x/r)^2 + 2 (x/r) - \tfrac 3 2 + \log r & x < r.
\end{cases}
$$
Then the solution to the weighted EL optimization problem \@ref(eq:elopt)-\@ref(eq:wel) is given by
\begin{equation}
\hat \omega_i = \frac{r_i}{1 - \hat \bla'\bg_i}, 
(\#eq:omegahat)
\end{equation}
where
\begin{equation}
\hat \bla = \argmax_{\bla} Q(\bla).
(\#eq:Qopt)
\end{equation}

<!-- \begin{equation} -->
<!-- \begin{aligned} -->
<!-- \hat \bla & = \argmax_{\bla} Q(\bla), \\ -->
<!-- Q(\bla) & = \sum_{i=1}^n r_i \log^\star\left(1 - \bla'\bg_i; r_i\right), \\ -->
<!-- \log^\star(x; r) & =  -->
<!-- \begin{cases}  -->
<!-- \log(x) & x \ge r \\ -->
<!-- - \tfrac 1 2 (x/r)^2 + 2 (x/r) - \tfrac 3 2 + \log r & x < r. -->
<!-- \end{cases} -->
<!-- \end{aligned} -->
<!-- (\#eq:optim) -->
<!-- \end{equation} -->

The convex optimization problem \@ref(eq:Qopt) can be solved by the Newton-Raphson algorithm.  That is, the Newton-Raphson updates are given by
$$
\bla_{t+1} = \bla_{t} - [Q_{(2)}(\bla_t)]^{-1} Q_{(1)}(\bla_t),
$$
where
\begin{equation}
\begin{aligned}
Q_{(1)}(\bla) = \frac{\ud}{\ud \bla} Q(\bla) & = -\sum_{i=1}^n r_i \log^\star_{(1)}(1 - \bla'\bg_i; r_i) \bg_i, \\
Q_{(2)}(\bla) = \frac{\ud^2}{\ud \bla \ud \bla'} Q(\bla) & = \sum_{i=1}^n r_i \log^\star_{(2)}(1 - \bla' \bg_i; r_i) \bg_i \bg_i',
\end{aligned}
(\#eq:nr)
\end{equation}

## Gradient

The gradient of the the weighted empirical loglikelihood with respect to $\tth$ is
$$
\begin{aligned}
\dth \log \EL(\tth) & = \dth \sum_{i=1}^n q_i \log \hat \omega_i(\tth) \\
& = \sum_{i=1}^n \frac{q_i}{1 - \bla'\bg_i} \cdot \dth \bla(\tth)'\bg_i(\tth) \\
& = R \times \left(\dth \bla(\tth)' \left[\sum_{i=1}^n \frac{r_i \cdot \bg_i(\tth)}{1 - \bla'\bg_i}\right] + \sum_{i=1}^n \hat \omega_i(\tth) \cdot \bla(\tth)' \dth \bg_i(\tth) \right),
\end{aligned}
$$
where $R = \sum_{i=1}^n q_i$.  Using \@ref(eq:omegahat), we have
$$
\sum_{i=1}^n \frac{r_i \cdot \bg_i}{1 - \hat \bla'\bg_i} = \sum_{i=1}^n \hat \omega_i \cdot \bg_i = \bz,
$$
where the second equality comes from the definition of the optimization constraint in \@ref(eq:elopt).  Therefore, the first term in the gradient disappears, such that we have
\begin{equation}
\dth \log \EL(\tth) = R \sum_{i=1}^n \hat \omega_i(\tth) \cdot \bla(\tth)' \dth \bg_i(\tth).
(\#eq:gradel)
\end{equation}

For automatic differentiation, it is useful to solve for $\frac{\ud}{\ud \bG} \log \EL(\bG)$, where $\bG_{n \times m} = (\bg_1, \ldots, \bg_n)$, in which case we have
\begin{equation}
\frac{\ud}{\ud \bG} \log \EL(\bG) = R \cdot \hat \oom_{n\times 1} \bla_{m\times 1}'.
(\#eq:gradelG)
\end{equation}


# Empirical Likelihood with Censoring

Consider the location-scale model
$$
y_i = \mu(\xx_i, \tth) + \sigma(\xx_i, \tth) + \eps_i,
$$
where $\xx_i \iid G(\xx)$, and independently $\eps_i \iid H(\eps)$ is a general noise distribution with $E[\eps] = 0$ and $\var(\eps) = 1$.  Suppose we observe $u_i = \min(y_i, c_i)$ where $c_i$ is the censoring time, and we also observe $\delta_i = \indicator\{y_i \le c_i\}$.  

Let 
$$
e_i = e_i(\tth) = \frac{u_i - \mu(\xx_i, \tth)}{\sigma(\xx_i, \tth}
$$
denote the censoring residuals.  Then for the moment conditions
$$
E[\bg(\xx, \eps, \tth)] = \bz,
$$
the EL with right censoring is defined as
\begin{equation}
\log \CEL(\tth) = \log \CEL(\tth, \hat{\oom}) = \sum_{i=1}^n \left[\delta_i \log(\hat\w_i) + (1-\delta_i) \log\left(\sum_{j=1}^n \indsmooth(e_i - e_j; s) \cdot \hat\w_j \right)\right],
\end{equation}
where $\indsmooth(\cdot; s)$ is the smoothed indicator function,
$$
\indsmooth(x; s) = \frac{1}{1 + \exp(s \cdot x)},
$$
and $\hat{\oom} = \hat{\oom}(\tth)$ solves the optimization problem
\begin{equation}
\max_{\oom} \log \CEL(\tth, \oom) \qquad \Big\vert \qquad \sum_{i=1}^n \omega_i \cdot \bg_i = \bz, \quad \oom \in \simplex^{n-1},
(\#eq:celopt)
\end{equation}
where $\bg_i = \bg(\xx_i, e_i, \tth)$.

## EM Algorithm

For fixed $\tth$, the CEL optimization problem \@ref(eq:celopt) can be solved via an EM algorithm.  The main steps are outlined here; details are provided in the Appendix.

- **Initial Step**

    Let $\oom_0 = (1/n, \ldots, 1/n)$.


- **E-Step** 

    Given $\oom_t$, calculate $q_i = \delta_i + \sum_{j=1}^n(1 - \delta_j) \cdot \tilde \omega_{ji}$, where
        $$
		\tilde \omega_{ij} = \frac{\indsmooth(e_i - e_j; s) \cdot \omega_{tj}}{\sum_{k=1}^n \indsmooth(e_i - e_k; s) \cdot \omega_{tk}}.
		$$
	
- **M-Step**

    Compute $\oom_{t+1}$ by solving the weighted EL problem \@ref(eq:elopt)-\@ref(eq:wel) with $q_i$ calculated as above.


# Appendix

Suppose we have $\eps_i \iid \categorical(\oom)$ and suppose that we have additional variables
$$
\tau_i \mid \{\eps_i = j\} \ind \bernoulli(p_{ij}).
$$
Thus, we have 
$$
\begin{aligned}
\tau_i & \ind \bernoulli(\sum_{j=1}^n p_{ij} \cdot \omega_j) \\
\eps_i \mid \{\tau_i = 1\} & \ind \categorical(\tilde \omega_{i1}, \ldots, \tilde \omega_{in}), \qquad \tilde \omega_{ij} = \frac{p_{ij} \cdot \omega_j}{\sum_{k=1}^n p_{ik} \cdot \omega_k}.
\end{aligned}
$$

Let $\indexset_k = \{i: \delta_i = k\}$ for $k = 0,1$, and similarly let $\eep_k = \{\eps_i: i \in \indexset_k\}$ and $\tta_k = \{\tau_i: i \in \indexset_k\}$.  Now suppose the $p_{ij}$ are known and we wish to estimate $\oom$ subject to the EL restriction
$$
\sum_{i=1}^n \omega_i \cdot \bg_i = \bz, \qquad \oom \in \simplex^{n-1}.
$$  
In the context of EM, the observed data is $(\eep_1 = \indexset_1, \tta_0 = \bm{1})$ and the missing data is $\eep_0$.  Thus, the complete data likelihood is
$$
\ell(\oom \mid \eep_0, \eep_1 = \indexset_1, \tta_0 = \bm{1}) = \sum_{i=1}^n \left[\delta_i \log \omega_i + (1-\delta_i) \sum_{j=1}^n \indicator\{\eps_i = j\} \cdot \log \omega_j\right],
$$
and the observed data likelihood is
$$
\ell(\oom \mid \eep_1 = \indexset_1, \tta_0 = \bm{1}) = \sum_{i=1}^n \left[\delta_i \log \omega_i + (1-\delta_i) \log \left(\sum_{j=1}^n p_{ij}\cdot\omega_j\right)\right].
$$

If at step $t$ of the EM algorithm we have $\oom_t$, the E-step consists of calculating
$$
\begin{aligned}
Q_t(\oom) & = E\left[\ell(\oom \mid \eep_0, \eep_1, \tta) \mid \eep_1 = \indexset_1, \tta = \bm{1}, \oom = \oom_t\right] \\
& = \sum_{i=1}^n \left[\delta_i \log \omega_i + (1-\delta_i)\sum_{j=1}^n E[\indicator\{\eps_1 = j\} \cdot \log \omega_j \mid \eep_1 = \indexset_1, \tta = \bm{1}, \oom = \oom_t] \right] \\
& = \sum_{i=1}^n \left[\delta_i \log \omega_i + (1-\delta_i)\sum_{j=1}^n \tilde \omega_{ij}^{(t)} \cdot \log \omega_j\right] \\
& = \sum_{i=1}^n q_i \log \omega_i,
\end{aligned}
$$
where $q_i = \delta_i + (1-\delta_i) \sum_{j=1}^n \tilde \omega_{ji}^{(t)}$ and
$$
\tilde \omega_{ij}^{(t)} = \frac{p_{ij} \cdot \omega_j^{(t)}}{\sum_{k=1}^n p_{ik} \cdot \omega_k^{(t)}}.
$$
The M-step of then consists of solving the weighted EL problem \@ref(eq:elopt)-\@ref(eq:wel) to obtain the new value of $\oom_{t+1}$ at step $t+1$.  Finally we recognize the specific case of the CEL optimization problem \@ref(eq:celopt) by setting $p_{ij} = \indsmooth(e_i - e_j; s)$.
